\documentclass[a4paper,12pt]{article}
\usepackage{amsmath}
\usepackage{amssymb}
\usepackage{geometry}
\geometry{a4paper, margin=1in}

\begin{document}

\title{Trigonometry Rules}
\author{}
\date{}
\maketitle

\section*{Basic Definitions}
\begin{itemize}
    \item \textbf{Sine:} \(\sin \theta = \frac{\text{opposite}}{\text{hypotenuse}}\)
    \item \textbf{Cosine:} \(\cos \theta = \frac{\text{adjacent}}{\text{hypotenuse}}\)
    \item \textbf{Tangent:} \(\tan \theta = \frac{\text{opposite}}{\text{adjacent}} = \frac{\sin \theta}{\cos \theta}\)
    \item \textbf{Cosecant:} \(\csc \theta = \frac{1}{\sin \theta}\)
    \item \textbf{Secant:} \(\sec \theta = \frac{1}{\cos \theta}\)
    \item \textbf{Cotangent:} \(\cot \theta = \frac{1}{\tan \theta} = \frac{\cos \theta}{\sin \theta}\)
\end{itemize}

\section*{Pythagorean Identities}
\begin{itemize}
    \item \(\sin^2 \theta + \cos^2 \theta = 1\)
    \item \(1 + \tan^2 \theta = \sec^2 \theta\)
    \item \(1 + \cot^2 \theta = \csc^2 \theta\)
\end{itemize}

\section*{Sum and Difference Formulas}
\begin{itemize}
    \item \(\sin(a \pm b) = \sin a \cos b \pm \cos a \sin b\)
    \item \(\cos(a \pm b) = \cos a \cos b \mp \sin a \sin b\)
    \item \(\tan(a \pm b) = \frac{\tan a \pm \tan b}{1 \mp \tan a \tan b}\)
\end{itemize}

\section*{Double Angle Formulas}
\begin{itemize}
    \item \(\sin(2\theta) = 2\sin \theta \cos \theta\)
    \item \(\cos(2\theta) = \cos^2 \theta - \sin^2 \theta = 2\cos^2 \theta - 1 = 1 - 2\sin^2 \theta\)
    \item \(\tan(2\theta) = \frac{2\tan \theta}{1 - \tan^2 \theta}\)
\end{itemize}

\section*{Half Angle Formulas}
\begin{itemize}
    \item \(\sin^2 \frac{\theta}{2} = \frac{1 - \cos \theta}{2}\)
    \item \(\cos^2 \frac{\theta}{2} = \frac{1 + \cos \theta}{2}\)
    \item \(\tan \frac{\theta}{2} = \frac{\sin \theta}{1 + \cos \theta} = \frac{1 - \cos \theta}{\sin \theta}\)
\end{itemize}

\section*{Product-to-Sum Formulas}
\begin{itemize}
    \item \(\sin a \sin b = \frac{1}{2}[\cos(a-b) - \cos(a+b)]\)
    \item \(\cos a \cos b = \frac{1}{2}[\cos(a-b) + \cos(a+b)]\)
    \item \(\sin a \cos b = \frac{1}{2}[\sin(a+b) + \sin(a-b)]\)
\end{itemize}

\section*{Sum-to-Product Formulas}
\begin{itemize}
    \item \(\sin a + \sin b = 2\sin\left(\frac{a+b}{2}\right)\cos\left(\frac{a-b}{2}\right)\)
    \item \(\sin a - \sin b = 2\cos\left(\frac{a+b}{2}\right)\sin\left(\frac{a-b}{2}\right)\)
    \item \(\cos a + \cos b = 2\cos\left(\frac{a+b}{2}\right)\cos\left(\frac{a-b}{2}\right)\)
    \item \(\cos a - \cos b = -2\sin\left(\frac{a+b}{2}\right)\sin\left(\frac{a-b}{2}\right)\)
\end{itemize}

\section*{Law of Sines and Law of Cosines}
\begin{itemize}
    \item \textbf{Law of Sines:} \(\frac{a}{\sin A} = \frac{b}{\sin B} = \frac{c}{\sin C}\)
    \item \textbf{Law of Cosines:} \(c^2 = a^2 + b^2 - 2ab\cos C\)
\end{itemize}

\end{document}
